simple conservativity theorem with diamond of multi-step beta as axiom

theories/SemiUnification/HOSemiU.v
@@ -16,7 +16,7 @@ Require Import Undecidability.SemiUnification.pts.
 
 (* 
   terms (according to pure type systems) 
-  P Q R ::= x | c | P Q| lambda x : P. Q | Pi x : P. Q 
+  P Q R ::= x | c | P Q | lambda (x : P). Q | Pi (x : P). Q 
   where x ranges over term variables and c ranges over term constants
 *)
 
@@ -25,13 +25,13 @@ Inductive step : term -> term -> Prop :=
   | step_beta P Q R: step (app (lam P Q) R) (subst_term (scons R var) Q) 
   | step_appL P P' Q: step P P' -> step (app P Q) (app P' Q)
   | step_appR P Q Q': step Q Q' -> step (app P Q) (app P Q')
-  | step_lamL P P' Q: step P P' -> step (lam P Q) (app P' Q)
-  | step_lamR P Q Q': step Q Q' -> step (lam P Q) (app P Q')
-  | step_piL P P' Q: step P P' -> step (pi P Q) (pi P' Q)
-  | step_piR P Q Q': step Q Q' -> step (pi P Q) (pi P Q').
+  | step_lamL P P' Q: step P P' -> step (lam P Q) (lam P' Q)
+  | step_lamR P Q Q': step Q Q' -> step (lam P Q) (lam P Q')
+  | step_PiL P P' Q: step P P' -> step (Pi P Q) (Pi P' Q)
+  | step_PiR P Q Q': step Q Q' -> step (Pi P Q) (Pi P Q').
 
-(* a term is in normal form if it is not reducible *)
-Definition normal_form (P : term) : Prop :=
+(* a term is normal (in normal form) if it is not reducible *)
+Definition normal (P : term) : Prop :=
   forall Q, not (step P Q).
 
 (* beta-equality is the reflexive, symmetric, transitive closure 
@@ -40,13 +40,14 @@ Definition eq_beta := clos_refl_sym_trans term step.
 
 Local Notation "P =β Q" := (eq_beta P Q) (at level 50).
 
-(* a normal valuation assigns formal forms to term variables *)
-Definition normal_valuation : Type := nat -> { P : term | normal_form P }.
+(* a valuation assigns terms with property p to term variables *)
+Definition valuation (p : term -> Prop) : Type := nat -> { P : term | p P }.
 
 (* substitution function "subst_term" is defined in pts.v *)
 
-(* replace free variables by assigned normal forms *)
-Definition substitute (φ : normal_valuation) (P : term) : term :=
+(* replace free variables by assigned terms with property p *)
+(* for example, p can be "normal_form" or "simple" *)
+Definition substitute {p : term -> Prop} (φ : valuation p) (P : term) : term :=
   subst_term (fun x => proj1_sig (φ x)) P.
 
 (* Higher-order Semi-unification Definition *)
@@ -54,28 +55,49 @@ Definition substitute (φ : normal_valuation) (P : term) : term :=
 (* inequality: s ≤ t *)
 Definition inequality : Type := (term * term).
 
-(* φ solves s ≤ t, if there is ψ such that ψ (φ (s)) =(beta) φ (s) *)
-Definition solution (φ : normal_valuation) : inequality -> Prop := 
-  fun '(s, t) => exists (ψ : normal_valuation), 
-    substitute ψ (substitute φ s) =β substitute φ t.
+(* φ solves s ≤ t, if there is ψ such that ψ (φ (s)) =β φ (s) *)
+(* property p in the range of φ is the same as in the range of ψ *)
+Definition solution {p : term -> Prop} (φ : valuation p) : inequality -> Prop := 
+  fun '(P, Q) => exists (ψ : valuation p), 
+    substitute ψ (substitute φ P) =β substitute φ Q.
 
 (* Higher-order Semi-unification *)
-(* is there a subnormal valuation φ that solves all inequalities? *)
-Definition HOSemiU (p: list inequality) := 
-  exists (φ: normal_valuation), forall (c: inequality), In c p -> solution φ c.
-
-
-
-
-
-
+(* is there a normal valuation φ that solves all inequalities? *)
+Definition HOSemiU (cs: list inequality) := 
+  exists (φ: valuation normal), forall (c: inequality), In c cs -> solution φ c.
 
 (* FACTS *)
 Require Import PeanoNat Lia.
 Require Import ssreflect ssrbool ssrfun.
 
+(* TODO part of autosubst? *)
+Lemma upRen_term_term_id x : upRen_term_term id x = x.
+Proof. by case: x. Qed.
 
-Definition term_norm := (compRen_term, renRen_term, rinstId_term, renComp_term).
+(* TODO autosubst? *)
+Lemma shift_up_term_term sigma x : (shift >> up_term_term sigma) x = (sigma >> ren_term shift) x.
+Proof. by case: x. Qed.
+
+(*TODO part of autosubst? no funext *)
+Lemma ren_term_id {P} : ren_term id P = P.
+Proof.
+  elim: P.
+  - done.
+  - done.
+  - by move=> /= ? -> ? ->.
+  - move=> /= ? -> ?.
+    under [ren_term (upRen_term_term id) _]extRen_term => ? do 
+      rewrite upRen_term_term_id.
+    by move=> ->.
+  - move=> /= ? -> ?.
+    under [ren_term (upRen_term_term id) _]extRen_term => ? do 
+      rewrite upRen_term_term_id.
+    by move=> ->.
+Qed.
+
+(* TODO rinstId_term uses funext, which is bad *)
+(* alternative: ren_term_id *)
+Definition term_norm := (compRen_term, renRen_term, @ren_term_id, renComp_term).
 
 (* such that simpl evaluates funcomp f g x *)
 Arguments funcomp {X Y Z} _ _ _ /.
@@ -89,7 +111,7 @@ Fixpoint allfv_term (p: nat -> Prop) (P: term) :=
   | const _ => True 
   | app P Q => allfv_term p P /\ allfv_term p Q
   | lam P Q => allfv_term p P /\ allfv_term (scons True p) Q
-  | pi P Q => allfv_term p P /\ allfv_term (scons True p) Q
+  | Pi P Q => allfv_term p P /\ allfv_term (scons True p) Q
   end.
 
 (* notion of a simple type represented by a term
@@ -101,49 +123,140 @@ Fixpoint simple (P: term) :=
   | const _ => False 
   | app P Q => False
   | lam P Q => False
-  | pi P Q => 
-      simple P /\ simple Q /\ 
-      allfv_term (fun y => 0 <> y) Q
+  | Pi P Q => (* Pi (x : P). Q is simple iff *)
+      simple P /\ (* P is simple *)
+      simple Q /\ (* Q is simple *)
+      allfv_term (fun y => 0 <> y) Q (* x does not occur free in Q *) 
   end.
 
-Axiom encode_term : term -> nat.
-Axiom decode_term : nat -> term.
-Axiom encode_decode_term : forall P, decode_term (encode_term P) = P.
+(* BEGIN term enumerability *)
 
-(* x does not occur in t *)
-Fixpoint fresh_inb (x: nat) (P: term) : bool := 
-  match P with
-  | var y => if Nat.eq_dec x y then false else true
-  | const _ => true 
-  | app P Q => fresh_inb x P && fresh_inb x Q
-  | lam P Q => fresh_inb x P && fresh_inb (S x) Q
-  | pi P Q => fresh_inb x P && fresh_inb (S x) Q
-  end.
+(* bijection from nat * nat to nat *)
+Definition encode_nat '(x, y) : nat := 
+  y + (nat_rec _ 0 (fun i m => (S i) + m) (y + x)).
 
-Lemma fresh_inbP {x P} : reflect (allfv_term (fun y => x <> y) P) (fresh_inb x P).
+(* bijection from nat to nat * nat *)
+Definition decode_nat (n : nat) : nat * nat := 
+  nat_rec _ (0, 0) (fun _ '(x, y) => if x is S x then (x, S y) else (S y, 0)) n.
+
+Lemma encode_nat_non_decreasing (x y: nat) : x + y <= encode_nat (x, y).
+Proof. elim: x=> [| x IH] /=; [| rewrite Nat.add_succ_r /=]; by lia. Qed.
+
+Lemma encode_decode_nat {xy: nat * nat} : decode_nat (encode_nat xy) = xy.
 Proof.
-Admitted.
+  move Hn: (encode_nat xy) => n. elim: n xy Hn.
+  { by move=> [[|?] [|?]]. }
+  move=> n IH [x [|y [H]]] /=.
+  { move: x => [|x [H]] /=; first done.
+    by rewrite (IH (0, x)) /= -?H ?PeanoNat.Nat.add_0_r. }
+  by rewrite (IH (S x, y)) /= -?H ?PeanoNat.Nat.add_succ_r.
+Qed.
+
+Opaque encode_nat decode_nat.
+
+(* injectively encode a term as a natural number *)
+Fixpoint encode_term (P: term) : nat :=
+  match P with
+  | var x => encode_nat (0, x)
+  | const c => encode_nat (1, c) 
+  | app P Q => encode_nat (2, (encode_nat (encode_term P, encode_term Q))) 
+  | lam P Q => encode_nat (3, (encode_nat (encode_term P, encode_term Q))) 
+  | Pi P Q => encode_nat (4, (encode_nat (encode_term P, encode_term Q))) 
+  end.
+
+Fixpoint decode_term' (k n: nat) : term :=
+  match k with
+  | 0 => var 0
+  | S k =>
+    match decode_nat n with
+    | (0, x) => var x
+    | (1, c) => const c
+    | (2, m) => let (m1, m2) := decode_nat m in
+      app (decode_term' k m1) (decode_term' k m2)
+    | (3, m) => let (m1, m2) := decode_nat m in
+      lam (decode_term' k m1) (decode_term' k m2)
+    | (4, m) => let (m1, m2) := decode_nat m in
+      Pi (decode_term' k m1) (decode_term' k m2)
+    | _ => var 0
+    end
+  end.
+
+(* uniquely decode a term from a natural number *)
+Definition decode_term (n: nat) := decode_term' (S n) n.
+
+Lemma encode_decode_term (P: term) : decode_term (encode_term P) = P.
+Proof.
+  rewrite /decode_term. 
+  suff : (forall k, encode_term P < k -> decode_term' k (encode_term P) = P) by apply.
+  move=> k. elim: k P; first by lia.
+  move=> k IH [] => /=.
+  - move=> ?. by rewrite encode_decode_nat.
+  - move=> ?. by rewrite encode_decode_nat.
+  - move=> P Q ?.
+    have ? := encode_nat_non_decreasing 2 (encode_nat (encode_term P, encode_term Q)).
+    have ? := encode_nat_non_decreasing (encode_term P) (encode_term Q).
+    rewrite ?encode_decode_nat. congr app; apply: IH; by lia.
+  - move=> P Q ?.
+    have ? := encode_nat_non_decreasing 3 (encode_nat (encode_term P, encode_term Q)).
+    have ? := encode_nat_non_decreasing (encode_term P) (encode_term Q).
+    rewrite ?encode_decode_nat. congr lam; apply: IH; by lia.
+  - move=> P Q ?.
+    have ? := encode_nat_non_decreasing 4 (encode_nat (encode_term P, encode_term Q)).
+    have ? := encode_nat_non_decreasing (encode_term P) (encode_term Q).
+    rewrite ?encode_decode_nat. congr Pi; apply: IH; by lia.
+Qed.
+
+Opaque encode_term decode_term.
+
+(* END term enumerability *)
+
+(* decidable equality on term *)
+Lemma term_eq_dec (P Q: term) : {P = Q} + {P <> Q}.
+Proof. by do 2 (decide equality). Qed. 
+
+(* decidable allfv_term on decidable predicates *)
+(* TODO move to autosubst? *)
+Lemma allfv_term_dec p P : (forall x, {p x} + {not (p x)}) ->
+  {allfv_term p P} + {not (allfv_term p P)}.
+Proof.
+  elim: P p.
+  - move=> >. by apply.
+  - move=> *. by left.
+  - move=> P IHP Q IHQ p Hp /=.
+    move: (IHP _ Hp) (IHQ _ Hp); clear; by firstorder done.
+  - move=> P IHP Q IHQ p Hp /=.
+    have H'p: forall x : nat, {(scons True p) x} + {not ((scons True p) x)} by (case; [left |]).
+    move: (IHP _ Hp) (IHQ _ H'p); clear; by firstorder done.
+  - move=> P IHP Q IHQ p Hp /=.
+    have H'p: forall x : nat, {(scons True p) x} + {not ((scons True p) x)} by (case; [left |]).
+    move: (IHP _ Hp) (IHQ _ H'p); clear; by firstorder done.
+Qed.
+
+Definition non_zero x := if x is 0 then False else True.
+
+Definition non_zero_dec x : {non_zero x} + {not (non_zero x)} :=
+  if x is 0 then right id else left I.
+
+(* decides whether 0 does not occur free in P *)
+Definition fresh_0 (P: term) := allfv_term_dec non_zero P non_zero_dec.
 
 (* make a term simple, remember non-simpel subterms as variables *)
 Fixpoint prune (xi: nat -> nat) (P: term) : term :=
   match P with
-  | pi P' Q' => 
-      if fresh_inb 0 Q' 
-        then pi (prune xi P') (ren_term shift (prune (scons 0 xi) Q'))
+  | Pi P' Q' => 
+      if fresh_0 Q' 
+        then Pi (prune xi P') (ren_term shift (prune (scons 0 xi) Q'))
         else var (encode_term (ren_term xi P))
   | _ => var (encode_term (ren_term xi P))
   end.
-
-
-
 
 (* remember non-simple subterms as distrinct variables 
 wrong because de Bruijn in prune Q' shifts variable names and rename before prune is not structural
 Fixpoint prune (P: term) :=
   match P with
-  | pi P' Q' => 
+  | Pi P' Q' => 
     if fresh_inb 0 Q' 
-      then pi (prune P') (ren_term S (prune Q')) 
+      then Pi (prune P') (ren_term S (prune Q')) 
       else var (encode_term P)
   | _ => var (encode_term P)
   end.
@@ -241,7 +354,7 @@ Proof.
   - move=> P IHP Q IHQ ? ? /= [/IHP -> HQ]. congr lam.
     apply: IHQ. apply: allfv_term_impl HQ. 
     case; [done | by move=> ? /= ->].
-  - move=> P IHP Q IHQ ? ? /= [/IHP -> HQ]. congr pi.
+  - move=> P IHP Q IHQ ? ? /= [/IHP -> HQ]. congr Pi.
     apply: IHQ. apply: allfv_term_impl HQ. 
     case; [done | by move=> ? /= ->].
 Qed.
@@ -258,7 +371,7 @@ Proof.
   - move=> P IHP Q IHQ ? ? /= [/IHP -> HQ]. congr lam.
     apply: IHQ. apply: allfv_term_impl HQ. 
     case; [done | by move=> ? /= ->].
-  - move=> P IHP Q IHQ ? ? /= [/IHP -> HQ]. congr pi.
+  - move=> P IHP Q IHQ ? ? /= [/IHP -> HQ]. congr Pi.
     apply: IHQ. apply: allfv_term_impl HQ. 
     case; [done | by move=> ? /= ->].
 Qed.
@@ -275,32 +388,49 @@ Proof.
 Qed.
 
 (* prune establishes simple *)
-Lemma prune_simple xi P : simple (prune xi P).
+Lemma simple_prune xi P : simple (prune xi P).
 Proof.
   elim: P xi => //=.
   move=> P IHP Q IHQ xi.
-  case HQ: (fresh_inb 0 Q); last done.
+  case: (fresh_0 Q) => ?; last done.
   constructor; [done | constructor].
   - by apply: simple_ren_term.
   - apply /allfv_ren_term. 
-    (* NOTE: assumption "fresh_inb 0 Q = true" was not used *)
     by apply: allfv_term_triv.
 Qed.
 
-(* extensionality principle for prune wrt. allfv *)
+(* extensionality principle for prune wrt. allfv_term *)
 Lemma ext_allfv_prune_term {zeta xi P} : 
   allfv_term (fun x => xi x = zeta x) P -> prune xi P = prune zeta P.
 Proof.
-Admitted.
+  elim: P xi zeta.
+  - by move=> /= > ->.
+  - done.
+  - move=> P IHP Q IHQ > /= [HP HQ].
+    congr (var (encode_term (app _ _))); by apply: ext_allfv_ren_term.
+  - move=> P IHP Q IHQ > /= [HP HQ].
+    congr (var (encode_term (lam _ _))); first by apply: ext_allfv_ren_term.
+    apply: ext_allfv_ren_term. apply: allfv_term_impl HQ.
+    case; [done | by move=> ? /= ->].
+  - move=> P IHP Q IHQ > /= [HP HQ].
+    case: (fresh_0 Q) => ? /=.
+    + congr Pi; first by apply: IHP.
+      congr ren_term. apply: IHQ.
+      apply: allfv_term_impl HQ. by case.
+    + congr (var (encode_term (Pi _ _))); first by apply: ext_allfv_ren_term.
+      apply: ext_allfv_ren_term. apply: allfv_term_impl HQ.
+      case; [done | by move=> ? /= ->].
+Qed.
 
-Lemma normal_formE {P} : normal_form P ->
+
+Lemma normalE {P} : normal P ->
   match P with
   | var _ => True
   | const _ => True 
   | app (lam _ _) _ => False
-  | app P Q => normal_form P /\ normal_form Q
-  | lam P Q => normal_form P /\ normal_form Q
-  | pi P Q => normal_form P /\ normal_form Q
+  | app P Q => normal P /\ normal Q
+  | lam P Q => normal P /\ normal Q
+  | Pi P Q => normal P /\ normal Q
   end.
 Proof.
 Admitted.
@@ -315,17 +445,16 @@ Proof.
     + by rewrite ?term_norm.
     + rewrite term_norm. apply: extRen_term. by case.
   - move=> P IHP Q IHQ ? ? /=.
-    case H1Q: (fresh_inb _ Q); case H'1Q: (fresh_inb _ _).
-    + congr pi; first done.
+    case: (fresh_0 Q) => H1Q; case: (fresh_0 _) => H'1Q.
+    + congr Pi; first done.
       congr ren_term. rewrite IHQ. apply: ext_allfv_prune_term.
       apply: allfv_term_triv. by case.
-    + exfalso. move: H'1Q => /fresh_inbP. apply.
-      apply /allfv_ren_term. move: H1Q => /fresh_inbP.
+    + exfalso. apply: H'1Q.
+      apply /allfv_ren_term. apply: allfv_term_impl H1Q. by case.
+    + exfalso. apply: H1Q.
+      move: H'1Q => /allfv_ren_term.
       apply: allfv_term_impl. by case.
-    + exfalso. move: H1Q => /fresh_inbP. apply.
-      move: H'1Q => /fresh_inbP /allfv_ren_term.
-      apply: allfv_term_impl. by case.
-    + congr (var (encode_term (pi _ _))); first by rewrite ?term_norm.
+    + congr (var (encode_term (Pi _ _))); first by rewrite ?term_norm.
       rewrite term_norm. apply: extRen_term. by case.
 Qed.
 
@@ -336,27 +465,20 @@ Lemma prune_subst_term {xi sigma P} : simple P -> prune xi (subst_term sigma P) 
 Proof.
   elim: P xi sigma => //=.
   move=> P IHP Q IHQ xi sigma.
-  move=> [HP] [H1Q H2Q]. case H3Q: (fresh_inb _ _).
-  - congr pi; first by apply: IHP.
+  move=> [HP] [H1Q H2Q]. case: (fresh_0 _) => H3Q.
+  - congr Pi; first by apply: IHP.
     rewrite (IHQ _ _ H1Q) term_norm.
     (* ext_term not applicable because substitutions are different on 0, which is absent *)
     apply: ext_allfv_subst_term.
     apply: allfv_term_impl H2Q.
     case; first done.
     move=> x _ /=. congr ren_term. by rewrite prune_ren_term.
-  - exfalso. move: H3Q => /fresh_inbP. apply.
+  - exfalso. apply: H3Q.
     rewrite allfv_subst_term. apply: allfv_term_impl H2Q.
     move=> [|? _] /=; first done.
     apply /allfv_ren_term. by apply: allfv_term_triv.
 Qed.
 
-(* TODO part of autosubst? *)
-Lemma upRen_term_term_id x : upRen_term_term id x = x.
-Proof. by case: x. Qed.
-
-(* TODO autosubst? *)
-Lemma shift_up_term_term sigma x : (shift >> up_term_term sigma) x = (sigma >> ren_term shift) x.
-Proof. by case: x. Qed.
 
 (* TODO autosubst? *)
 Lemma ext_ren_term' {xi zeta P Q} : 
@@ -369,145 +491,78 @@ Lemma up_ren_subst_term_term' xi sigma x:
   (upRen_term_term xi >> up_term_term sigma) x = up_term_term (xi >> sigma) x.
 Proof. by apply: up_ren_subst_term_term. Qed.
 
-(* x is fresh in P iff x renamed to any z does not change P *)
-Lemma fresh_inbP' x P : fresh_inb x P = true <-> 
-  (forall z, ren_term (Nat.iter x upRen_term_term (scons z shift)) P = P).
-Proof.
-  rewrite -/(is_true _) -(rwP fresh_inbP). elim: P x.
-  - move=> y x /=. admit.
-  - done.
-  - admit.
-  - move=> P IHP Q IHQ x /=. constructor.
-    + move=> [HP HQ] z. congr lam.
-      * by apply /(iffLR (IHP x)).
-      * have -> := iffLR (IHQ (S x)) _ z; last done.
-        apply: allfv_term_impl HQ.
-        case; first done.
-        move=> ? /=. by lia.
-    + move=> H. constructor.
-      * apply /(iffRL (IHP x)) => z.
-        by case: (H z).
-      * have := iffRL (IHQ (S x)). admit. (* easy *)
-Admitted.
-
-(* x is fresh in P iff there is room to shift variable names to/from x *)
-Lemma fresh_inbP'' x P : fresh_inb x P = true <-> 
-  (P = ren_term (Nat.iter x upRen_term_term shift) 
-        (ren_term (Nat.iter x upRen_term_term (scons 0 id)) P)).
-Proof.
-  elim: P x.
-  - move=> y x /=. constructor.
-    + case: (Nat.eq_dec x y); first done.
-      move=> /= Hxy _. congr var.
-      elim: x y Hxy; first by case.
-      move=> x IH [|y]; first done.
-      move=> ? /=. congr S. apply: IH. by lia.
-    + case: (Nat.eq_dec x y); last done.
-      move=> /= <- []. elim: x; first done.
-      by move=> x IH /= [].
-  - done.
-  - move=> P IHP Q IHQ x /=. constructor.
-    + by move=> /andP => - [/IHP <-] /IHQ <-.
-    + by move=> [/IHP -> /IHQ ->].
-  - move=> P IHP Q IHQ x /=. constructor.
-    + by move=> /andP => - [/IHP <-] /IHQ <-.
-    + by move=> [/IHP -> /(IHQ (S x)) ->].
-  - move=> P IHP Q IHQ x /=. constructor.
-    + by move=> /andP => - [/IHP <-] /IHQ <-.
-    + by move=> [/IHP -> /(IHQ (S x)) ->].
-Qed.
-
-(* 0 is fresh in P if P is some shifted term Q *)
-Corollary fresh_inb0P'' P : fresh_inb 0 P = true <-> 
-  (exists Q, P = ren_term shift Q).
-Proof.
-  rewrite fresh_inbP'' /=. constructor.
-  - move=> ->. by eexists.
-  - move=> [Q] ->.  rewrite ?term_norm.
-    apply: extRen_term. by case.
-Qed.
-
-Lemma fN_fresh_inbI (fN : term -> term) {P} :
-  (forall P', fN (ren_term shift P') = ren_term shift (fN P')) ->
-  fresh_inb 0 P = true -> fresh_inb 0 (fN P) = true.
-Proof.
-  move=> HfN /fresh_inb0P'' => - [Q ->].
-  apply /fresh_inb0P''. exists (fN Q).
-  by rewrite HfN.
-Qed.
-
 Lemma up_term_term_funcomp {xi sigma x} : 
   up_term_term (xi >> sigma) x = (upRen_term_term xi >> up_term_term sigma) x.
 Proof.
   by case: x.
 Qed.
 
-(* pruning intanciated pruned instance (?) *)
-(* "KEY LEMMA 2", tau is the resulting simple substitution *)
-(* NOTE: fN is the relevant normalizer, xi3 = xi1 = id *)
-Lemma key2 {fN : term -> term} {sigma xi1 xi3 P} : 
-  (* fN preserves pi *)
-  (forall P' Q', fN (pi P' Q') = pi (fN P') (fN Q')) ->
-  (* fN preserves shifts; strong assumption *)
-  (forall P', fN (ren_term shift P') = ren_term shift (fN P')) ->
-  (* resulting simple valuation *)
-  let tau := (fun x => ren_term xi3 (prune id (fN (subst_term sigma (decode_term x))))) in
-  (* homomorphism *)
-  subst_term tau (prune xi1 P) = ren_term xi3 (prune id (fN (subst_term (funcomp sigma xi1) P))).
-Proof.
-  move=> H1fN H2fN tau. subst tau.
-  elim: P xi1 xi3 sigma.
-  - move=> > /=. by rewrite encode_decode_term.
-  - move=> > /=. by rewrite encode_decode_term.
-  - move=> * /=. by rewrite encode_decode_term /= ?term_norm.
-  - move=> P IHP Q IHQ xi1 xi3 sigma /=. rewrite encode_decode_term /= ?term_norm /=.
-    congr (ren_term xi3 (prune id (fN (lam _ _)))). apply: ext_term. by case.
-    (* case pi P Q *)
-  - move=> P IHP Q IHQ xi1 xi3 sigma /=.
-    case HQ: (fresh_inb 0 Q).
-    (* case (var 0) does not occur in Q *)
-    + rewrite H1fN /=.
-
-    have -> : fresh_inb 0 (fN (subst_term (up_term_term (funcomp sigma xi1)) Q)) = true.
-    { apply: fN_fresh_inbI; first done.
-      apply /fresh_inbP. move: HQ => /fresh_inbP.
-      rewrite allfv_subst_term. apply: allfv_term_impl.
-      move=> [|? _ /=]; [done | ]. rewrite allfv_ren_term.
-      by apply: allfv_term_triv. }
-      move=> /=. congr pi; first done.
-      rewrite term_norm.
-      under [subst_term _ (prune _ Q)]ext_term => ? do 
-        rewrite shift_up_term_term /funcomp term_norm.
-      rewrite IHQ term_norm. apply: ext_ren_term'; first by case.
-
-      have ->: subst_term (up_term_term (xi1 >> sigma)) Q = 
-        ren_term shift (subst_term ((0 .: xi1) >> sigma) Q).
-      { rewrite term_norm. apply: ext_allfv_subst_term.
-        move: HQ => /fresh_inbP. apply: allfv_term_impl. by case. }
-      by rewrite H2fN prune_ren_term.
-    (* case (var 0) occurs in Q *)
-    + rewrite /= encode_decode_term /= ?term_norm.
-      under [subst_term (up_term_term _) _]ext_term => ?
-        do rewrite -up_ren_subst_term_term'.
-      done.
-Qed.
-
 Fixpoint simple_map_term (f: term -> term) (P: term) : term :=
   match P with
-  | pi P' Q' => 
-      if fresh_inb 0 Q' 
-        then pi (simple_map_term f P') 
+  | Pi P' Q' => 
+      if fresh_0 Q' 
+        then Pi (simple_map_term f P') 
           (ren_term shift (simple_map_term ((ren_term (scons 0 id)) >> f) Q'))
         else f P
   | _ => f P
   end.
 
-Lemma simple_map_ren_term {f xi P} : 
-  simple_map_term f (ren_term xi P)  = simple_map_term (ren_term xi >> f) P.
+Lemma ext_simple_map_term {f g P} : (forall P', f P' = g P') -> 
+  simple_map_term f P = simple_map_term g P.
 Proof.
-  elim: P f xi.
-  - done.
-Admitted.
+  elim: P f g.
+  - move=> >. by apply.
+  - move=> >. by apply.
+  - move=> P IHP Q IHQ f g. by apply.
+  - move=> P IHP Q IHQ f g. by apply.
+  - move=> P IHP Q IHQ f g Hfg /=.
+    case: (fresh_0 Q) => HQ /=; last done.
+    congr Pi; first by apply IHP.
+    congr ren_term. apply: IHQ. by move=> P' /=.
+Qed.
+
+Lemma ren_simple_map_term {xi f P} : 
+  ren_term xi (simple_map_term f P) = simple_map_term (f >> ren_term xi) P.
+Proof.
+  elim: P xi f => //.
+  move=> P IHP Q IHQ xi f /=.
+  case: (fresh_0 Q) => HQ /=; last done.
+  congr Pi; first done.
+  rewrite term_norm ?IHQ. apply: ext_simple_map_term => ?.
+  rewrite /= term_norm. apply: extRen_term.
+  by case.
+Qed.
+
+(* TODO part of autosubst standard file *)
+Lemma funcomp_assoc {X1 X2 X3 X4} {f : X1 -> X2} {g : X2 -> X3} {h : X3 -> X4} : 
+  funcomp h (funcomp g f) = funcomp (funcomp h g) f.
+Proof. reflexivity. Qed.
+
+Lemma simple_map_ren_term {f xi P} : 
+  simple_map_term f (ren_term xi P) = simple_map_term (ren_term xi >> f) P.
+Proof.
+  elim: P f xi => //.
+  move=> P IHP Q IHQ f xi /=.
+  case: (fresh_0 Q) => HQ /=.
+  - case: (fresh_0 _) => H'Q /=; first last.
+    { exfalso. apply: H'Q. rewrite allfv_ren_term.
+      apply: allfv_term_impl HQ. by case. }
+    congr Pi; first by apply: IHP.
+    congr ren_term. rewrite IHQ.
+    have /ext_simple_map_term -> : forall P', 
+      (ren_term (upRen_term_term xi) >> (ren_term (scons 0 id) >> f)) P' = 
+      (ren_term (upRen_term_term xi >> (scons 0 id)) >> f) P'.
+    { move=> ? /=. by rewrite term_norm. }
+    have /ext_simple_map_term -> : forall P',
+      (ren_term (0 .: id) >> (ren_term xi >> f)) P' =
+      (ren_term ((0 .: id) >> xi) >> f) P'.
+    { move=> ? /=. by rewrite term_norm. }
+    rewrite -?IHQ. congr simple_map_term.
+    apply: ext_allfv_ren_term. apply: allfv_term_impl HQ. by case.
+  - case: (fresh_0 _) => H'Q /=; last done.
+    exfalso. apply: HQ. move: H'Q. rewrite allfv_ren_term.
+    apply: allfv_term_impl. by case.
+Qed.
 
 (* pruning intanciated pruned instance (?) *)
 (* "KEY LEMMA 2", tau is the resulting simple substitution *)
@@ -526,28 +581,27 @@ Proof.
   - move=> * /=. by rewrite encode_decode_term /= ?term_norm.
   - move=> P IHP Q IHQ xi1 xi3 sigma /=. rewrite encode_decode_term /= ?term_norm /=.
     congr (ren_term xi3 (prune id (simple_map_term fN (lam _ _)))). apply: ext_term. by case.
-    (* case pi P Q *)
+    (* case Pi P Q *)
   - move=> P IHP Q IHQ xi1 xi3 sigma /=.
-    case HQ: (fresh_inb 0 Q).
+    case: (fresh_0 Q) => HQ /=.
     (* case (var 0) does not occur in Q *)
-    + have -> : fresh_inb 0 (subst_term (up_term_term (xi1 >> sigma)) Q) = true.
-      { apply /fresh_inbP. move: HQ => /fresh_inbP.
-        rewrite allfv_subst_term. apply: allfv_term_impl.
+    + case: (fresh_0 _) => H'Q /=; first last.
+      { exfalso. apply: H'Q. rewrite allfv_subst_term.
+        apply: allfv_term_impl HQ. 
         move=> [|x _ /=]; first done.
         rewrite allfv_ren_term. apply: allfv_term_triv. by case. }
-      move=> /=.
-      set b := (fresh_inb 0 _). have ->: b = true.
-      { subst b. apply /fresh_inbP. rewrite allfv_ren_term. 
+      case: (fresh_0 _) => H''Q /=; first last.
+      { exfalso. apply: H''Q. rewrite allfv_ren_term.
         apply: allfv_term_triv. by case. }
-      move=> /=. congr pi; first done.
+      congr Pi; first done.
       rewrite ?term_norm. rewrite prune_ren_term.
-      have -> : (↑ >> (0 .: id)) = id by done.
+      have -> : (↑ >> (scons 0 id)) = id by done.
       under [subst_term _ (prune _ Q)]ext_term => ? do 
         rewrite shift_up_term_term /funcomp term_norm.
       rewrite IHQ. apply: ext_ren_term'; first by case.
       rewrite -simple_map_ren_term term_norm. congr (prune id (simple_map_term fN _)). 
-      apply: ext_allfv_subst_term. move: HQ => /fresh_inbP.
-      apply: allfv_term_impl => - [|? _ /=]; first done.
+      apply: ext_allfv_subst_term.
+      apply: allfv_term_impl HQ => - [|? _ /=]; first done.
       by rewrite ?term_norm.
     (* case (var 0) occurs in Q *)
     + rewrite /= encode_decode_term /= ?term_norm.
@@ -565,101 +619,259 @@ Corollary key2'_final {fN : term -> term} {sigma P} :
   let tau := (fun x => prune id (simple_map_term fN (subst_term sigma (decode_term x)))) in
   (* homomorphism *)
   subst_term tau (prune id P) = prune id (simple_map_term fN (subst_term sigma P)).
-Proof. have := @key2' fN sigma id id P. by rewrite /= term_norm. Qed.
+Proof. 
+  have := @key2' fN sigma id id P.
+  rewrite /= ?term_norm.
+  move=> <-. apply: ext_term => ?. by rewrite ?term_norm.
+Qed.
 
 Definition red_beta := clos_refl_trans term step.
 
-Lemma term_eq_dec (P Q: term) : {P = Q} + {P <> Q}.
-Proof. by do 2 (decide equality). Qed. 
 
-Lemma ext_simple_map_term {f g P} : (forall P', f P' = g P') -> 
-  simple_map_term f P = simple_map_term g P.
+
+(* TODO part of autosubst? *)
+(* all free variables are left unchanged by a renaming *)
+Lemma ren_term_allfv_id {xi P} : allfv_term (fun x => xi x = x) P -> ren_term xi P = P.
 Proof.
-  elim: P f g.
-  - move=> >. by apply.
-  - move=> >. by apply.
-  - move=> P IHP Q IHQ f g. by apply.
-  - move=> P IHP Q IHQ f g. by apply.
-  - move=> P IHP Q IHQ f g Hfg /=. 
-    case HQ: (fresh_inb 0 Q); last done.
-    congr pi; first by apply IHP.
-    congr ren_term. apply: IHQ. by move=> P' /=.
+  move=> H. rewrite -[RHS]ren_term_id.
+  by apply: ext_allfv_ren_term.
 Qed.
-
+ 
 Lemma simple_map_term_id {P} : 
   simple_map_term id P = P.
 Proof.
   elim: P => //.
-  move=> P IHP Q IHQ /=. case HQ: (fresh_inb 0 Q); last done.
-  congr pi; first done.
-Admitted.
+  move=> P IHP Q IHQ /=. case: (fresh_0 Q) => HQ /=; last done.
+  congr Pi; first done.
+  rewrite ren_simple_map_term.
+  rewrite -simple_map_ren_term.
+  have ->: ren_term shift = (ren_term shift) >> id by done.
+  rewrite -simple_map_ren_term term_norm.
+  rewrite ren_term_allfv_id; last done.
+  apply: allfv_term_impl HQ. by case.
+Qed.
 
 Lemma simple_map_simple_map_term {f g P} :
   simple_map_term g (simple_map_term f P) = simple_map_term (f >> simple_map_term g) P.
 Proof.
   elim: P f g => //.
-  move=> P IHP Q IHQ f g /=. case HQ: (fresh_inb 0 Q); last done.
-  rewrite /=. set b := (fresh_inb 0 _).
-  have ->: b = true.
-  { subst b. apply /fresh_inbP. rewrite allfv_ren_term.
+  move=> P IHP Q IHQ f g /=.
+  case: (fresh_0 Q) => HQ /=; last done.
+  case: (fresh_0 _) => H'Q /=; first last.
+  { exfalso. apply: H'Q. rewrite allfv_ren_term.
     apply: allfv_term_triv. by case. }
-  congr pi; first done.
+  congr Pi; first done.
   congr ren_term. rewrite simple_map_ren_term IHQ.
   apply: ext_simple_map_term => ? /=.
   apply: ext_simple_map_term => ? /=.
   by rewrite ?term_norm.
 Qed.
 
-Lemma red_beta_piI {P Q P' Q'} : 
-  red_beta P P' -> red_beta Q Q' -> red_beta (pi P Q) (pi P' Q').
-Proof.
-Admitted.
-
 Lemma red_beta_diamond {P Q1 Q2} : red_beta P Q1 -> red_beta P Q2 -> 
   { Q | red_beta Q1 Q /\ red_beta Q2 Q }.
 Proof.
 Admitted.
 
+Definition rt_rt1n := Relations.Operators_Properties.clos_rt_rt1n_iff.
+Arguments rt_step {A R x y}.
+
+(* TODO move to red_beta facts *)
+Lemma red_beta_appI P P' Q Q' : red_beta P P' -> red_beta Q Q' -> red_beta (app P Q) (app P' Q').
+Proof.
+  move=> /rt_rt1n H. elim: H Q Q'.
+  - move=> >. elim => *.
+    + apply: rt_step. by apply: step_appR.
+    + by apply: rt_refl.
+    + apply: rt_trans; by eassumption.
+  - move=> > ? ? IH > /IH ?.
+    apply: rt_trans; last by eassumption.
+    apply: rt_step. by apply: step_appL.
+Qed.
+
+(* TODO move to red_beta facts *)
+Lemma red_beta_lamI P P' Q Q' : red_beta P P' -> red_beta Q Q' -> red_beta (lam P Q) (lam P' Q').
+Proof.
+  move=> /rt_rt1n H. elim: H Q Q'.
+  - move=> >. elim => *.
+    + apply: rt_step. by apply: step_lamR.
+    + by apply: rt_refl.
+    + apply: rt_trans; by eassumption.
+  - move=> > ? ? IH > /IH ?.
+    apply: rt_trans; last by eassumption.
+    apply: rt_step. by apply: step_lamL.
+Qed.
+
+
+(* TODO move to red_beta facts *)
+Lemma red_beta_PiI P P' Q Q' : red_beta P P' -> red_beta Q Q' -> red_beta (Pi P Q) (Pi P' Q').
+Proof.
+  move=> /rt_rt1n H. elim: H Q Q'.
+  - move=> >. elim => *.
+    + apply: rt_step. by apply: step_PiR.
+    + by apply: rt_refl.
+    + apply: rt_trans; by eassumption.
+  - move=> > ? ? IH > /IH ?.
+    apply: rt_trans; last by eassumption.
+    apply: rt_step. by apply: step_PiL.
+Qed.
+
+(* TODO move to beta facts *)
+Lemma step_betaI {P Q R R'} : R' = (subst_term (scons R var) Q) -> step (app (lam P Q) R) R'.
+Proof. move=> ->. by apply: step_beta. Qed.
+
+(* TODO move to beta facts *)
+Lemma step_ren_termI xi {P Q} : step P Q -> step (ren_term xi P) (ren_term xi Q).
+Proof.
+  move=> H. elim: H xi; [|by eauto using step with nocore ..].
+  move=> > /=. apply: step_betaI. rewrite ?term_norm.
+  apply: ext_term. by case.
+Qed.
+
+(* TODO move to beta facts *)
+Lemma red_beta_ren_termI xi {P Q} : red_beta P Q -> red_beta (ren_term xi P) (ren_term xi Q).
+Proof.
+  elim.
+  - move=> *. by apply /rt_step /step_ren_termI.
+  - move=> *. by apply: rt_refl.
+  - move=> *. apply: rt_trans; by eassumption.
+Qed.
+
 Lemma simple_map_term_red_beta_impl {f g P} : (forall P', red_beta (f P') (g P')) ->
   red_beta (simple_map_term f P) (simple_map_term g P).
 Proof.
-Admitted.
-
-Lemma ren_simple_map_term {xi f P} : 
-  ren_term xi (simple_map_term f P) = simple_map_term (f >> ren_term xi) P.
-Proof.
-  elim: P xi f => //.
-  move=> P IHP Q IHQ xi f /=.
-  case HQ: (fresh_inb 0 Q); last done.
-  move=> /=. congr pi; first done.
-  rewrite term_norm ?IHQ. apply: ext_simple_map_term => ?.
-  rewrite /= term_norm. apply: extRen_term.
-  by case.
+  elim: P f g.
+  - move=> >. by apply.
+  - move=> >. by apply.
+  - move=> P IHP Q IHQ ? ?. by apply.
+  - move=> P IHP Q IHQ ? ?. by apply.
+  - move=> P IHP Q IHQ ? ? H /=.
+    case: (fresh_0 Q) => HQ /=; last by apply: H.
+    apply: red_beta_PiI; first by apply: IHP.
+    apply: red_beta_ren_termI. apply: IHQ.
+    move=> ?. by apply: H.
 Qed.
 
-Lemma red_beta_ren_termI xi {P Q} : red_beta P Q -> red_beta (ren_term xi P) (ren_term xi Q).
+Lemma step_allfv_term_impl {p P Q} : step P Q -> allfv_term p P -> allfv_term p Q.
 Proof.
-Admitted.
+  move=> H. elim: H p; [| by firstorder done ..].
+  move=> > /= [[_ +] ?]. rewrite allfv_subst_term.
+  apply: allfv_term_impl. by case.
+Qed.
 
-Lemma red_beta_allfv_termI {p P Q} : red_beta P Q -> allfv_term p P -> allfv_term p Q.
+Lemma red_beta_allfv_term_impl {p P Q} : red_beta P Q -> allfv_term p P -> allfv_term p Q.
 Proof.
-Admitted.
+  elim.
+  - move=> >. by apply: step_allfv_term_impl.
+  - done.
+  - by move=> > _ IH1 _ IH2 /IH1.
+Qed.
+
+(*
+(* alternative formulation of red_beta *)
+Inductive red_beta' : term -> term -> Prop :=
+  | red_beta_refl P : red_beta' P P
+  | red_beta_contract P P1 P2 Q Q': 
+      red_beta' P (app (lam P1 P2) Q) -> red_beta' (subst_term (scons P2 var) Q) Q' -> red_beta' (app P Q) Q'
+  | red_beta_app P P' Q Q': red_beta' P P' -> red_beta' Q Q' -> red_beta' (app P Q) (app P' Q')
+  | red_beta_lam P P' Q Q': red_beta' P P' -> red_beta' Q Q' -> red_beta' (lam P Q) (lam P' Q')
+  | red_beta_Pi P P' Q Q': red_beta' P P' -> red_beta' Q Q' -> red_beta' (Pi P Q) (Pi P' Q').
+*)
+
+(* TODO move to red_beta facts *)
+Lemma red_beta_subst_termI {sigma tau P} : (forall x, red_beta (sigma x) (tau x)) -> 
+  red_beta (subst_term sigma P) (subst_term tau P).
+Proof.
+  elim: P sigma tau.
+  - move=> >. by apply.
+  - move=> *. by apply: rt_refl.
+  - move=> P IHP Q IHQ sigma tau H /=.
+    apply: red_beta_appI; [by apply: IHP | by apply: IHQ].
+  - move=> P IHP Q IHQ sigma tau H /=.
+    apply: red_beta_lamI; first by apply IHP.
+    apply: IHQ. case; first by apply: rt_refl.
+    move=> x /=. by apply: red_beta_ren_termI.
+  - move=> P IHP Q IHQ sigma tau H /=.
+    apply: red_beta_PiI; first by apply IHP.
+    apply: IHQ. case; first by apply: rt_refl.
+    move=> x /=. by apply: red_beta_ren_termI.
+Qed.
+
+Lemma red_betaE {P Q} : red_beta P Q ->
+  match P with
+  | var _ => Q = P
+  | const _ => Q = P
+  | app P1 P2 => 
+      (exists Q1 Q2, Q = app Q1 Q2 /\ red_beta P1 Q1 /\ red_beta P2 Q2) \/
+      (exists P11 P12, red_beta P1 (lam P11 P12) /\ red_beta (subst_term (scons P2 var) P12) Q)
+  | lam P1 P2 => exists Q1 Q2, Q = lam Q1 Q2 /\ red_beta P1 Q1 /\ red_beta P2 Q2
+  | Pi P1 P2 => exists Q1 Q2, Q = Pi Q1 Q2 /\ red_beta P1 Q1 /\ red_beta P2 Q2
+  end.
+Proof.
+  move=> /rt_rt1n. elim.
+  - case.
+    + done.
+    + done.
+    + move=> ? ?. left. 
+      do 2 eexists. constructor; first by reflexivity.
+      constructor; by apply: rt_refl.
+    + move=> ? ?. 
+      do 2 eexists. constructor; first by reflexivity.
+      constructor; by apply: rt_refl.
+    + move=> ? ?. 
+      do 2 eexists. constructor; first by reflexivity.
+      constructor; by apply: rt_refl.
+  - move=> > [].
+    + move=> > ? _. right. 
+      do 2 eexists. constructor; first by apply: rt_refl.
+      by apply /rt_rt1n.
+    + move=> > ? _ [].
+      * move=> [?] [?] [->] [? ?]. left.
+        do 2 eexists. constructor; first by reflexivity.
+        constructor; last done.
+        apply: rt_trans; last by eassumption.
+        by apply: rt_step.
+      * move=> [?] [?] [?] ?. subst. right.
+        do 2 eexists. constructor; last by eassumption.
+        by apply: rt_trans; [apply: rt_step | by eassumption].
+    + move=> > ? _ [].
+      * move=> [?] [?] [->] [? ?]. left.
+        do 2 eexists. constructor; first by reflexivity.
+        constructor; first done.
+        apply: rt_trans; last by eassumption.
+        by apply: rt_step.
+      * move=> [?] [?] [?] ?. subst. right.
+        do 2 eexists. constructor; first by eassumption.
+        apply: rt_trans; last by eassumption.
+        apply: red_beta_subst_termI. case; first by apply: rt_step.
+        move=> *. by apply: rt_refl.
+    + move=> > /rt_step ? _ [?] [?] [->] [? ?].
+      do 2 eexists. constructor; first by reflexivity.
+      by constructor; first by (apply: rt_trans; eassumption).
+    + move=> > /rt_step ? _ [?] [?] [->] [? ?].
+      do 2 eexists. constructor; first by reflexivity.
+      by constructor; last by (apply: rt_trans; eassumption).
+    + move=> > /rt_step ? _ [?] [?] [->] [? ?].
+      do 2 eexists. constructor; first by reflexivity.
+      by constructor; first by (apply: rt_trans; eassumption).
+    + move=> > /rt_step ? _ [?] [?] [->] [? ?].
+      do 2 eexists. constructor; first by reflexivity.
+      by constructor; last by (apply: rt_trans; eassumption).
+Qed.
+
 
 (* pruning intanciated pruned instance (?) *)
 (* "KEY LEMMA 3", fN is the relevant normalizer *)
 (* to use with "key2'_final" *)
-Lemma construct_fN xi P Q : red_beta P Q -> 
+Lemma construct_fN xi {P Q} : red_beta P Q -> 
   exists (fN : term -> term), 
     red_beta (ren_term xi Q) (simple_map_term fN (ren_term xi P)) /\
     (forall R, red_beta R (fN R)).
 Proof.
   elim: P xi Q.
-  - move=> x xi Q HQ. exists id. rewrite simple_map_term_id. constructor.
-    + apply: red_beta_ren_termI. admit. (* easy by NF *)
-    + move=> ?. by apply: rt_refl.
-  - move=> c xi Q HQ. exists id. rewrite simple_map_term_id. constructor.
-    + apply: red_beta_ren_termI. admit. (* easy by NF *)
-    + move=> ?. by apply: rt_refl.
+  - move=> x xi Q /red_betaE HQ. exists id. rewrite simple_map_term_id HQ.
+     constructor => *; by apply: rt_refl.
+  - move=> c xi Q /red_betaE HQ. exists id. rewrite simple_map_term_id HQ.
+    constructor => *; by apply: rt_refl.
   - move=> P IHP Q IHQ xi R HR.
     exists (fun R' => if term_eq_dec R' (ren_term xi (app P Q)) then (ren_term xi R) else R').
     constructor.
@@ -679,26 +891,25 @@ Proof.
           by apply: red_beta_ren_termI.
         * move=> /= _. by apply: rt_refl.
   - move=> P IHP Q IHQ xi R HR /=.
-    case HQ: (fresh_inb 0 _).
-    + have : exists P' Q', R = pi P' Q' /\ (red_beta P P') /\ (red_beta Q Q') by admit. (* easy by NF *)
-      move=> [P'] [Q'] [->] [HPP' HQQ'].
+    case: (fresh_0 _) => HQ /=.
+    + move: HR => /red_betaE - [P'] [Q'] [->] [HPP' HQQ'].
       have [fNP [H1fNP H2fNP]] := IHP xi _ HPP'.
       have [fNQ [H1fNQ H2fNQ]] := IHQ (scons 0 xi) _ HQQ'.
       exists (fun R' => sval (red_beta_diamond (H2fNP R') (H2fNQ R'))).
       constructor.
-      * rewrite /=. apply: red_beta_piI.
+      * rewrite /=. apply: red_beta_PiI.
         ** apply: rt_trans; first by eassumption.
            apply: simple_map_term_red_beta_impl => R'.
            by move: (sval _) (svalP (red_beta_diamond (H2fNP R') (H2fNQ R'))) => ? [].
         ** have ->: ren_term (upRen_term_term xi) Q' = ren_term shift (ren_term (0 .: xi) Q').
            { rewrite term_norm. apply: ext_allfv_ren_term.
-             apply: red_beta_allfv_termI; first by eassumption.
-             move: HQ => /fresh_inbP. rewrite allfv_ren_term.
+             apply: red_beta_allfv_term_impl; first by eassumption.
+             move: HQ. rewrite allfv_ren_term.
              apply: allfv_term_impl. by case. }
             apply: red_beta_ren_termI.
 
             rewrite -simple_map_ren_term term_norm.
-            have HH : forall x, (upRen_term_term xi >> (0 .: id)) x = (0 .: xi) x.
+            have HH : forall x, (upRen_term_term xi >> (scons 0 id)) x = (scons 0 xi) x.
             by case.
             under [ren_term _ Q]extRen_term => ? do rewrite HH.
 
@@ -709,165 +920,150 @@ Proof.
         move: (sval _) (svalP (red_beta_diamond (H2fNP R') (H2fNQ R'))) => R'' [? _].
         apply: rt_trans; last by eassumption.
         by apply: H2fNP.
-    + exists (fun R' => if term_eq_dec R' (ren_term xi (pi P Q)) then (ren_term xi R) else R').
+    + exists (fun R' => if term_eq_dec R' (ren_term xi (Pi P Q)) then (ren_term xi R) else R').
     constructor.
     * move=> /=. case: (term_eq_dec _ _) => /=; last done.
       move=> _. by apply: rt_refl.
-    * move=> ?. case: (term_eq_dec _ _).
-      ** move=> /= ->. rewrite -/(ren_term xi (pi _ _)).
-        by apply: red_beta_ren_termI.
-      ** move=> /= _. by apply: rt_refl.
-Admitted.
+    * move=> ?. case: (term_eq_dec _ _); last by (move=> *; apply: rt_refl).
+      move=> /= ->. by apply: (red_beta_ren_termI xi HR).
+Qed.
 
-
-
-(* maybe needs CPS renaming *)
-(* interesting case only for single beta step*)
-Lemma construct_fN P Q : red_beta P Q -> 
-  exists (fN : term -> term), 
-    red_beta Q (simple_map_term fN P) /\
-    (forall R, red_beta R (fN R)).
+Corollary construct_fN' {P Q} : red_beta P Q -> normal Q ->
+  exists (fN : term -> term), simple_map_term fN P = Q.
 Proof.
-  elim: P Q.
-  - move=> x Q HQ. exists id. rewrite simple_map_term_id. admit.
-  - move=> c Q HQ. exists id. rewrite simple_map_term_id. admit.
-  - move=> P IHP Q IHQ R HR.
-    exists (fun R' => if term_eq_dec R' (app P Q) then R else R').
-    constructor.
-    + move=> /=. case: (term_eq_dec _ _); last done.
-      move=> /= _. by apply: rt_refl.
-    + move=> ?. case: (term_eq_dec _ _).
-      * by move=> /= ->.
-      * move=> /= _. by apply: rt_refl.
-  - move=> P IHP Q IHQ R HR.
-    exists (fun R' => if term_eq_dec R' (lam P Q) then R else R').
-    constructor.
-    + move=> /=. case: (term_eq_dec _ _); last done.
-      move=> /= _. by apply: rt_refl.
-    + move=> ?. case: (term_eq_dec _ _).
-      * by move=> /= ->.
-      * move=> /= _. by apply: rt_refl.
-  - move=> P IHP Q IHQ R HR.
-    case HQ: (fresh_inb 0 Q).
-    + have : exists P' Q', R = pi P' Q' /\ (red_beta P P') /\ (red_beta Q Q') by admit.
-      move=> [P'] [Q'] [->] [HPP' HQQ'].
-      have [fNP [H1fNP H2fNP]] := IHP _ HPP'.
-      have [fNQ [H1fNQ H2fNQ]] := IHQ _ HQQ'.
-      exists (fun R' => sval (red_beta_diamond (H2fNP R') (H2fNQ R'))).
-      constructor.
-      * rewrite /= HQ. apply: red_beta_piI.
-        ** apply: rt_trans; first by eassumption.
-           apply: simple_map_term_red_beta_impl => R'.
-           by move: (sval _) (svalP (red_beta_diamond (H2fNP R') (H2fNQ R'))) => ? [].
-        ** apply: rt_trans; first by eassumption.
-          have ->: Q = var 1 by admit.
-          simpl. ?????????
-        rewrite -simple_map_ren_term.
-           rewrite ren_simple_map_term.
-           rewrite -simple_map_ren_term.
-  
-           apply: simple_map_term_red_beta_impl => R' /=.
-           move: (sval _) (svalP (red_beta_diamond (H2fNP (ren_term (0 .: id) R')) (H2fNQ (ren_term (0 .: id) R')))) => ? [].
-           move=> _ /(red_beta_ren_termI shift).
-           congr red_beta.
-           NOOOOO simple with renaming but no fnq?
-          admit.
-      * move=> R'.
-        move: (sval _) (svalP (red_beta_diamond (H2fNP R') (H2fNQ R'))) => R'' [? _].
-        apply: rt_trans; last by eassumption.
-        by apply: H2fNP.
-    + exists (fun R' => if term_eq_dec R' (pi P Q) then R else R').
-      constructor.
-      + move=> /=. case: (term_eq_dec _ _); last done.
-        move=> /= _. by apply: rt_refl.
-      + move=> ?. case: (term_eq_dec _ _).
-        * by move=> /= ->.
-        * move=> /= _. by apply: rt_refl.
+  move=> /(construct_fN id) - [fN] [H1Q _] H2Q.
+  exists fN. move: H1Q. rewrite /red_beta ?term_norm /=. 
+  move: (simple_map_term _ _) => ? /rt_rt1n. case; first done.
+  by move=> > /H2Q.
+Qed.
 
+Lemma stepE {P Q} : step P Q -> 
+  match P with
+  | var _ => False
+  | const _ => False
+  | app P1 P2 => 
+    (exists P11 P12, P1 = lam P11 P12 /\ Q = subst_term (scons P2 var) P12) \/
+    (exists Q1, Q = app Q1 P2 /\ step P1 Q1) \/
+    (exists Q2, Q = app P1 Q2 /\ step P2 Q2)
+  | lam P1 P2 => 
+      (exists Q1, Q = lam Q1 P2 /\ step P1 Q1) \/
+      (exists Q2, Q = lam P1 Q2 /\ step P2 Q2)
+  | Pi P1 P2 => 
+      (exists Q1, Q = Pi Q1 P2 /\ step P1 Q1) \/
+      (exists Q2, Q = Pi P1 Q2 /\ step P2 Q2)
+  end.
+Proof. case; by eauto. Qed.
 
-(* interesting case only for single beta step*)
-Lemma construct_fN P Q : red_beta P Q -> 
-  exists (fN : term -> term), red_beta Q (simple_map_term fN P).
+Lemma normal_PiI {P Q} : normal P -> normal Q -> normal (Pi P Q).
+Proof. move=> HP HQ R /stepE. by case => - [?] [_] => [/HP | /HQ]. Qed.
+
+Lemma normal_varI {x} : normal (var x).
+Proof. by move=> ? /stepE. Qed. 
+
+(* construct a valuation from a substitution sigma which pointwise satisfied predicate p *)
+Definition valuationI (p: term -> Prop)
+  (sigma: nat -> term) (H: forall x, p (sigma x)) : valuation p :=
+  (fun x => exist _ _ (H x)).
+
+Lemma normal_ren_termE xi {P} : normal (ren_term xi P) -> normal P.
+Proof. by move=> HP Q /(step_ren_termI xi) /HP. Qed.
+
+Lemma normal_simple_substituteI {φ: valuation normal} {P} : simple P -> normal (substitute φ P).
 Proof.
-  elim: P Q.
-  - move=> x Q ?. exists (fun=> Q). by apply: rt_refl.
-  - move=> c Q ?. exists (fun=> Q). by apply: rt_refl.
-  - move=> P IHP Q IHQ R.
-    exists (fun=> R). by apply: rt_refl.
-  - move=> P IHP Q IHQ R.
-    exists (fun=> R). by apply: rt_refl.
-  - move=> P IHP Q IHQ R HPQ.
-    case HQ: (fresh_inb 0 Q).
-    + have : exists P' Q', R = pi P' Q' /\ (red_beta P P') /\ (red_beta Q Q') by admit.
-      move=> [P'] [Q'] [->] [HPP' HQQ'].
-      have [fNP HfNP] := IHP _ HPP'.
-      have [fNQ HfNQ] := IHQ _ HQQ'.
-      exists (fun R' => if term_eq_dec P R' then P' else Q').
-      rewrite /= HQ. apply: red_beta_piI => /=.
-      * ??? 
-    + exists (fun=> R) => /=. rewrite HQ. by apply: rt_refl.
+  elim: P φ => //.
+  - move=> x φ _. rewrite /substitute /=.
+    by apply: svalP.
+  - move=> P IHP Q IHQ φ /= [/IHP {}IHP] [/IHQ {}IHQ] HQ.
+    rewrite /substitute /=. apply: normal_PiI; first by apply: IHP.
+    set sigma := up_term_term (fun x => sval (φ x)).
+    apply: (IHQ (valuationI normal sigma _)).
+    move=> [|x]; first by apply: normal_varI.
+    apply: (normal_ren_termE (scons 0 id)) => /=.
+    rewrite ?term_norm. by apply: svalP.
+Qed.
 
+Definition rst_rst1n := Operators_Properties.clos_rst_rst1n_iff.
 
-  move HP: (P) => R.
-  elim: R P Q HP.
-  - move=> x P Q HP ?.
-    exists (fun _ => Q).
-    by apply: rt_refl.
-  - admit.
-  -
-
-  elim: P Q.
-  - move=> *. exists id. rewrite simple_map_term_id. admit. (* Q is var n *)
-  - admit.
-  - move=> P IHP Q IHQ R.
-
-
-
-(* interesting case only for single beta step*)
-Lemma construct_fN P Q : red_beta P Q -> 
-  exists (fN : term -> term), red_beta Q (simple_map_term fN P).
+Lemma red_beta_normal {P Q} : red_beta P Q -> normal P -> P = Q.
 Proof.
-  elim.
-  - admit.
-  - move=> ?. exists id. admit. (* easy *)
-  - move=> {}P {}Q R _ [fNPQ HfNPQ] _ [fNQR HfNQR].
-    exists (funcomp (simple_map_term fNQR) fNPQ) => /=.
-    apply: rt_trans; first by eassumption.
-    rewrite -simple_map_simple_map_term.
+  case /rt_rt1n; first done.
+  by move=> > + _ H => /H.
+Qed.
 
-
-
-(*
-(* interesting case only for single beta step*)
-Lemma construct_fN P Q : red_beta P Q -> 
-  exists (fN : term -> term), 
-    fN P = Q /\
-    (forall P' Q', fN (pi P' Q') = pi (fN P') (fN Q')) /\
-    (forall P', fN (ren_term shift P') = ren_term shift (fN P')).
+Lemma eq_beta_normal {P Q} : normal Q -> P =β Q -> red_beta P Q.
 Proof.
-  elim.
-  - admit.
-  - move=> ?. by exists id.
-  - move=> {}P {}Q R _ [fNPQ] [<-] [H1fNPQ H2fNPQ] _ [fNQR] [<-] [H1fNQR H2fNQR].
-    exists (funcomp fNQR fNPQ) => /=. constructor; first done.
-    constructor; by congruence.
-Admitted.
-*)
+  move=> HQ /rst_rst1n HPQ. 
+  elim: HPQ HQ; first by (move=> *; apply: rt_refl).
+  move=> {}P R {}Q [|].
+  - move=> /rt_step ? _ IH ?. 
+    apply: rt_trans; [by eassumption | by apply: IH].
+  - move=> /rt_step HRP _ IH HQ.
+    have [Q' [HPQ' /red_beta_normal HQQ']] := red_beta_diamond HRP (IH HQ).
+    by rewrite (HQQ' HQ).
+Qed.
+
+(* anny solution φ to a simple instance (P, Q) entails a simple solution sigma' *)
+Lemma simple_solutionI {φ ψ: valuation normal} {P Q} : simple P -> simple Q -> 
+  substitute ψ (substitute φ P) =β substitute φ Q ->
+  let sigma' := (fun x => prune id (sval (φ x))) in
+  exists tau', 
+    (forall x, simple (tau' x)) /\
+    subst_term tau' (subst_term sigma' P) = subst_term sigma' Q.
+Proof.
+  move=> H1P H1Q HPQ sigma'.
+  have H2Q : normal (substitute φ Q).
+  { by apply: normal_simple_substituteI. }
+
+  have H'PQ : red_beta (substitute ψ (substitute φ P)) (substitute φ Q).
+  { by apply: eq_beta_normal. }
+
+  have [fN HfN] := construct_fN' H'PQ H2Q.
+  exists (fun x => prune id (simple_map_term fN (substitute ψ (decode_term x)))).
+  constructor.
+  - move=> ?. by apply: simple_prune.
+  - subst sigma'. rewrite /substitute in HfN.
+    rewrite -(prune_subst_term H1P).
+    rewrite -(prune_subst_term H1Q).
+    rewrite -HfN.
+    by rewrite -key2'_final.
+Qed.
+
+(* a list of simple inequalities has a solution iff it has a simple solution *)
+Theorem simple_convervativity (cs: list inequality) : 
+  (* every inequality is simple *)
+  (Forall (fun '(P, Q) => simple P /\ simple Q) cs) -> 
+  (* cs has a normal solution *)
+  HOSemiU cs ->
+  (* cs has a simple solution *)
+  exists (φ: valuation simple), forall (c: inequality), In c cs -> solution φ c.
+Proof.
+  move=> Hcs [φ /Forall_forall Hφ].
+  unshelve eexists (valuationI simple (fun x => prune id (sval (φ x))) _).
+  - move=> ? /=. by apply: simple_prune.
+  - apply /Forall_forall.
+    apply: Forall_impl (Forall_and Hcs Hφ).
+    move=> [P Q] [[HP HQ]] [ψ] /(simple_solutionI HP HQ) /=.
+    move=> [tau'] [Htau' H].
+    exists (valuationI _ _ Htau').
+    rewrite /substitute /valuationI /= H.
+    by apply: rst_refl.
+Qed.
+
+Print Assumptions simple_convervativity.
 
 (* EXPERIMENTAL *)
 
-
-(* EXPLICIT Pi-K APPROACH, arr is pi P Q such that 0 is fresh in Q *)
+(* EXPLICIT Pi-K APPROACH, arr is Pi P Q such that 0 is fresh in Q *)
 (* NOT NEEDED ?*)
 (*
-(* store pimple type information up to a term leaf *)
+(* store Pimple type information up to a term leaf *)
 Inductive term' := 
   | atom : term -> term'
   | arr : term' -> term' -> term'.
 
 Fixpoint simplify (xi: nat -> nat) (P: term) : term' :=
   match P with
-  | pi P' Q' => 
+  | Pi P' Q' => 
       if fresh_inb 0 Q' 
         then arr (simplify xi P') (simplify (scons 0 xi) Q')
         else atom P
@@ -879,7 +1075,7 @@ Fixpoint simplify (xi: nat -> nat) (P: term) : term' :=
 Fixpoint prune2 (P: term') : term' :=
   match P with
   | atom P' => atom (var ())
-  | pi P' Q' => 
+  | Pi P' Q' => 
       if fresh_inb 0 Q' 
         then SemiU.arr (prune2 xi P') (prune2 (scons 0 xi) Q')
         else SemiU.atom (encode_term (ren_term xi P))
@@ -897,7 +1093,7 @@ Lemma normal_formE {P} : normal_form P ->
   | app (lam _ _) _ => False
   | app P Q => normal_form P /\ normal_form Q
   | lam P Q => normal_form P /\ normal_form Q
-  | pi P Q => normal_form P /\ normal_form Q
+  | Pi P Q => normal_form P /\ normal_form Q
   end.
 Proof.
   elim: P.
@@ -922,7 +1118,7 @@ Fixpoint is_normal_form (P : term) : bool :=
   | app (lam _ _) _ => false
   | app P Q => is_normal_form P && is_normal_form Q
   | lam P Q => is_normal_form P && is_normal_form Q
-  | pi P Q => is_normal_form P && is_normal_form Q
+  | Pi P Q => is_normal_form P && is_normal_form Q
   end.
 
 
@@ -940,57 +1136,4 @@ Proof.
     Search reflect.
     
     constructor.
-*)
-*)
-
-
-
-(* SIMPLE SemiU APPROACH FAILS *)
-
-(*
-
-Require Undecidability.SemiUnification.SemiU.
-
-(* make a term simple, remember non-simpel subterms as variables *)
-Fixpoint prune2 (xi: nat -> nat) (P: term) : SemiU.term :=
-  match P with
-  | pi P' Q' => 
-      if fresh_inb 0 Q' 
-        then SemiU.arr (prune2 xi P') (prune2 (scons 0 xi) Q')
-        else SemiU.atom (encode_term (ren_term xi P))
-  | _ => SemiU.atom (encode_term (ren_term xi P))
-  end.
-
-(* pruning intanciated pruned instance (?) *)
-(* "KEY LEMMA 2", tau is the resulting simple substitution *)
-(* NOTE: fN is the relevant normalizer, xi3 = xi1 = id *)
-Lemma key2_2 {fN : term -> term} {sigma xi1 xi2 P} : 
-  (* fN preserves pi *)
-  (forall P' Q', fN (pi P' Q') = pi (fN P') (fN Q')) ->
-  (* fN preserves shifts; strong assumption *)
-  (forall P', fN (ren_term shift P') = ren_term shift (fN P')) ->
-  (* resulting simple valuation *)
-  let tau := (fun x => prune2 xi2 (fN (subst_term sigma (decode_term x)))) in
-  (* homomorphism *)
-  SemiU.substitute tau (prune2 xi1 P) = prune2 xi2 (fN (subst_term (funcomp sigma xi1) P)).
-Proof.
-  move=> H1fN H2fN tau. subst tau.
-  elim: P xi1 xi2 sigma.
-  - move=> > /=. by rewrite encode_decode_term.
-  - move=> > /=. by rewrite encode_decode_term.
-  - move=> * /=. by rewrite encode_decode_term /= ?term_norm.
-  - move=> P IHP Q IHQ xi1 xi2 sigma /=. rewrite encode_decode_term /= ?term_norm /=.
-    congr (prune2 xi2 (fN (lam _ _))). apply: ext_term. by case.
-    (* case pi P Q *)
-  - move=> P IHP Q IHQ xi1 xi2 sigma /=.
-    case HQ: (fresh_inb 0 Q).
-    (* case (var 0) does not occur in Q *)
-    + rewrite H1fN /=.
-
-    have -> : fresh_inb 0 (fN (subst_term (up_term_term (funcomp sigma xi1)) Q)) = true.
-    { admit. }
-    move=> /=. congr SemiU.arr; first done.
-
-    under [subst_term _ Q]ext_term => ? do rewrite up_term_term_funcomp.
-    rewrite -IHQ.
 *)
